examples/scache/ArrayPtr.s.dfy
@@ -5,7 +5,7 @@ module Ptrs {
 
   datatype Ptr = Ptr(_internal: PtrInternalOpaqueType)
 
-  function method nullptr() : Ptr
+  function method {:extern} nullptr() : Ptr
 
   // Ghosty
 
@@ -15,22 +15,8 @@ module Ptrs {
   // Normal ptrs
 
   datatype Deref<V> = Deref(ptr: Ptr, v: V)
-  datatype ConstDeref<V> = ConstDeref(ptr: Ptr, v: V)
 
-  // linear Deref
-  // linear ConstDeref
-
-  // linear Deref
-  // readonly-linear Deref
-
-  // ptr p
-  // Deref(p, 5)
-  //
-  // var x := read(p, deref)
-  // x == 5
-  //
-
-  method {:extern} ptr_write<V>(p: Ptr, v: V, inout linear d: Deref<V>)
+  method {:extern} ptr_write<V>(p: Ptr, inout linear d: Deref<V>, v: V)
   requires old_d.ptr == p
   ensures d.ptr == p
   ensures d.v == v
@@ -40,23 +26,9 @@ module Ptrs {
   requires d.ptr == p
   ensures v == d.v
 
-  /*method {:extern} ptr_const_read<V>(p: Ptr, shared d: ConstDeref<V>)
-  returns (v: V)
-  requires d.ptr == p
-  ensures v == d.v*/
-
-
   // Array ptrs
 
-  datatype R<V> =
-    | ArrayReadCount(ptr: Ptr, s: seq<V>, refcount: int)
-    | ConstArrayDeref(ptr: Ptr, s: seq<V>)
-
-  type ArrayDeref<V> = r: R<V> | r.ArrayReadCount? && r.refcount == 0
-      witness ArrayReadCount(nullptr(), [], 0)
-
-  type ConstArrayDeref<V> = r: R<V> | r.ConstArrayDeref?
-      witness ConstArrayDeref(nullptr(), [])
+  datatype ArrayDeref<V> = ArrayDeref(ptr: Ptr, s: seq<V>)
 
   method {:extern} array_write<V>(p: Ptr, linear inout d: ArrayDeref, i: int, v: V)
   requires old_d.ptr == p
@@ -69,34 +41,7 @@ module Ptrs {
   requires 0 <= i < |d.s|
   ensures v == d.s[i]
 
-  method {:extern} const_array_read<V>(p: Ptr, shared d: ConstArrayDeref<V>, i: int)
-  returns (v: V)
-  requires d.ptr == p
-  requires 0 <= i < |d.s|
-  ensures v == d.s[i]
+  // Read-only
 
-  predicate transform<V(!new)>(a: multiset<R<V>>, b: multiset<R<V>>)
-  {
-    || (exists ptr, s, refcount ::
-      && a == multiset{ArrayReadCount(ptr, s, refcount)}
-      && b == multiset{ArrayReadCount(ptr, s, refcount + 1), ConstArrayDeref(ptr, s)}
-    )
-    || (exists ptr, s, refcount, s' ::
-      && a == multiset{ArrayReadCount(ptr, s, refcount), ConstArrayDeref(ptr, s')}
-      && b == multiset{ArrayReadCount(ptr, s, refcount - 1)}
-    ) 
-  }
-
-  /*method main(p: Ptr, linear d: ArrayDeref<int>)
-  returns (linear d': ArrayDeref<int>)
-  requires |d.s| == 1
-  requires d.ptr == p
-  {
-    var a := array_read(p, d, 0);
-    d' := d;
-  }*/
-
-  // forall C, D . rel(C, D) ==> exists C', D' . (A+C) ==> (A'+C') & (B+D) ==> (B'+D') & rel(C',D')
-  // ------
-  // A+B ==> A'+B'
+  datatype Const<A> = Const(a: A)
 }
